Fixed unsound axiom in Random.v and all specs and proofs that were relying on it.

src/Random.v
@@ -633,19 +633,19 @@ Qed.
    assumptions about them *)
 Axiom randomRBool : bool * bool -> RandomSeed -> bool * RandomSeed.
 Axiom randomRBoolCorrect :
-  forall b b1 b2,
-    implb b1 b = true /\ implb b b2 = true <->
-    exists seed, (fst (randomRBool (b1, b2) seed)) = b.
-Axiom randomRNat  : nat  * nat  -> RandomSeed -> nat * RandomSeed.
+  forall b b1 b2, implb b1 b2 ->
+    (implb b1 b && implb b b2 <->
+    exists seed, (fst (randomRBool (b1, b2) seed)) = b).
+Axiom randomRNat  : nat  * nat -> RandomSeed -> nat * RandomSeed.
 Axiom ramdomRNatCorrect:
-  forall n n1 n2,
-    n1 <= n /\ n <= n2 <->
-    exists seed, (fst (randomRNat (n1, n2) seed)) = n.
+  forall n n1 n2, n1 <= n2 ->
+    (n1 <= n <= n2 <->
+    exists seed, (fst (randomRNat (n1, n2) seed)) = n).
 Axiom randomRInt  : Z * Z    -> RandomSeed -> Z * RandomSeed.
 Axiom ramdomRIntCorrect:
-  forall z z1 z2,
-    Z.leb z1 z /\ Z.leb z z2 <->
-    exists seed, (fst (randomRInt (z1, z2) seed)) = z.
+  forall z z1 z2, Z.leb z1 z2 ->
+    (Z.leb z1 z && Z.leb z z2 <->
+    exists seed, (fst (randomRInt (z1, z2) seed)) = z).
 
 
 (* A small experiment showing that infinite random trees
@@ -719,8 +719,9 @@ Class Random (A : Type)  :=
     super :> OrdType A;
     randomR : A * A -> RandomSeed -> A * RandomSeed;
     randomRCorrect :
-      forall (a a1 a2 : A), leq a1 a /\ leq a a2 <->
-                            exists seed, fst (randomR (a1, a2) seed) = a
+      forall (a a1 a2 : A), leq a1 a2 ->
+      (leq a1 a && leq a a2 <->
+       exists seed, fst (randomR (a1, a2) seed) = a)
   }.
 
 Program Instance RandomBool : Random bool :=
